

$$\lim_{x \rightarrow -1} \frac{x+1}{\sqrt[3]{x}+1} \cdot \frac{(\sqrt[3]{x})^2 - \sqrt[3]{x} + 1}{(\sqrt[3]{x})^2 - \sqrt[3]{x} + 1} = (*)$$

$$\sqrt[3]{-1} = -1$$

$$a^3 + b^3 = (a+b)(a^2 - ab + b^2) \quad \bullet \quad a = \sqrt[3]{x}, \quad b = 1$$

$$a^2 - b^2 = (a+b)(a-b)$$

$$(*) = \lim_{x \rightarrow -1} \frac{\cancel{(x+1)}((\sqrt[3]{x})^2 - \sqrt[3]{x} + 1)}{\cancel{(x+1)}} = (\sqrt[3]{-1})^2 - \sqrt[3]{-1} + 1 =$$

$$= (-1)^2 - (-1) + 1 = 3$$

$$\bullet \lim_{x \rightarrow 0} \frac{\sqrt{1+x} - \sqrt{1-x}}{x} \cdot \frac{\sqrt{1+x} + \sqrt{1-x}}{\sqrt{1+x} + \sqrt{1-x}} =$$

$$= \lim_{x \rightarrow 0} \frac{1+x - (1-x)}{x \cdot (\sqrt{1+x} + \sqrt{1-x})} = \lim_{x \rightarrow 0} \frac{1+x - 1+x}{x(\sqrt{1+x} + \sqrt{1-x})} =$$

$$= \lim_{x \rightarrow 0} \frac{2x}{x(\sqrt{1+x} + \sqrt{1-x})} = \frac{2}{1+1} = 1$$

$$(1+x)^a = 1 + ax + \frac{a(a-1)}{2} x^2 + o(x^2) \quad \left| \sqrt{1+x} = (1+x)^{\frac{1}{2}} \right.$$

$$\bullet \lim_{x \rightarrow 0} \frac{\sqrt{1+x} - \sqrt{1-x}}{x} = \lim_{x \rightarrow 0} \frac{1 + \frac{1}{2}x + o(x) - (1 + \frac{1}{2}(-x) + o(x))}{x} =$$

$$= \lim_{x \rightarrow 0} \frac{\frac{1}{2}x + \frac{1}{2}x + o(x)}{x} = \lim_{x \rightarrow 0} \frac{\cancel{x} \left(1 + \frac{o(x)}{x}\right)^{o}}{\cancel{x}} = 1$$

$$\lim_{x \rightarrow 0} \frac{e^{1-\cos(x)} - e^{\sin(x)}}{\log(1+3x)} = (\star)$$

$$\cos(x) = 1 - \frac{x^2}{2} + \frac{x^4}{4!} + o(x^4)$$

$$\sin(x) = x - \frac{x^3}{6} + o(x^3)$$

$$\log(1+x) = x - \frac{x^2}{2} + o(x^2) \quad \bigg| \quad \log(1+3x) = 3x - \frac{(3x)^2}{2} + o(x^2)$$

$$e^x = 1 + x + \frac{x^2}{2} + \frac{x^3}{6} + o(x^3)$$

$$(\star) = \lim_{x \rightarrow 0} \frac{e^{1 - (1 - \frac{x^2}{2} + o(x^4))} - e^{x + o(x)}}{3x + o(x)} =$$

$$= \lim_{x \rightarrow 0} \frac{e^{\frac{x^2}{2} + o(x^2)} - e^{x + o(x)}}{3x + o(x)} =$$

$$= \lim_{x \rightarrow 0} \frac{1 + \frac{x^2}{2} + o(x^2) - (1 + x + o(x))}{3x + o(x)} =$$

$$= \lim_{x \rightarrow 0} \frac{\frac{x^2}{2} + o(x^2) - x + o(x)}{3x + o(x)} = \lim_{x \rightarrow 0} \frac{-x + o(x)}{3x + o(x)}$$

$$= \lim_{x \rightarrow 0} \frac{-1 + \frac{o(x)}{x}}{3 + \frac{o(x)}{x}} = -\frac{1}{3}$$

$$x^n \in o(x^m) \text{ se } n > m \quad (\text{per } x \rightarrow 0)$$

$$3x^2 + o(x) = o(x)$$

$$f(x) \in o(g(x)) \Leftrightarrow \lim_{x \rightarrow 0} \frac{f(x)}{g(x)} = 0$$

$$\sin(x) = x + o(x) = x + f(x) \quad \text{con } f(x) \in o(x)$$

$$\lim_{x \rightarrow 0} \frac{o(x)}{x} = 0$$

$$\lim_{x \rightarrow 0} \frac{e^{\sin(x)} - \log(1+x) - 1}{x^2} =$$

$$= \lim_{x \rightarrow 0} \frac{e^{x+o(x)} - (x+o(x)) - 1}{x^2} =$$

$$= \lim_{x \rightarrow 0} \frac{1 + x + o(x) - x + o(x) - 1}{x^2} = \lim_{x \rightarrow 0} \frac{o(x)}{x^2} \quad ??$$

$$\left[\begin{array}{l} o(x) + o(x) \in o(x) \\ o(x) - o(x) \in o(x) \end{array} \right]$$

$$\lim_{x \rightarrow 0} \frac{e^{x+o(x)} - \left(x - \frac{x^2}{2} + o(x^2)\right) - 1}{x^2} = (\star)$$

$$= \lim_{x \rightarrow 0} \frac{1 + x + o(x) - x + \frac{x^2}{2} + o(x^2) - 1}{x^2} =$$

$$= \lim_{x \rightarrow 0} \frac{o(x)}{x^2} \quad ??$$

$$(\star) = \lim_{x \rightarrow 0} \frac{1 + x + \frac{x^2}{2} + o(x^2) - \left(x - \frac{x^2}{2} + o(x^2)\right) - 1}{x^2} =$$

$$= \lim_{x \rightarrow 0} \frac{x^2 + o(x^2)}{x^2} = 1$$

$$x^2 + \overbrace{2x o(x)}^{e o(x^2)} + o(x^2)$$

$$e^{x+o(x)} = 1 + (x+o(x)) + \frac{(x+o(x))^2}{2} + o((x+o(x))^2) =$$

$$e^x = 1 + x + \frac{x^2}{2} + o(x^2)$$

$$= 1 + x + o(x) + \frac{x^2}{2} + o(x^2) + o(x^2)$$

$$= 1 + x + o(x)$$

$$\sin(x) = x + o(x) \stackrel{!}{=} x + o(x^2)$$

$$\sin(x) = x - \frac{x^3}{6} + o(x^3)$$

$$\cos(x) = 1 - \frac{x^2}{2} + o(x^2) = 1 - \frac{x^2}{2} + o(x^3)$$

$$\cos(x) = 1 - \frac{x^2}{2} + \frac{x^4}{4!} + o(x^4)$$

• $x^2 \in o(x) \Rightarrow x^2 \rightarrow o(x)$

$$\lim_{x \rightarrow 0} \frac{x^2}{x} \stackrel{!!}{=} 0$$

$$\lim_{x \rightarrow 0} \frac{x^2}{x} = \lim_{x \rightarrow 0} x = 0$$

• Sviluppare fino al terzo ordine

$$e^{x+x^2} \quad | \quad e^x = 1 + x + \frac{x^2}{2} + \frac{x^3}{6} + o(x^3)$$

$$e^{x+x^2} = 1 + x + x^2 + \frac{(x+x^2)^2}{2} + \frac{(x+x^2)^3}{6} + o((x+x^2)^3)$$

$$e^{x+x^2} = 1 + x + x^2 + o(x+x^2) = 1 + x + x^2 + o(x) = 1 + x + o(x)$$

$$\begin{aligned} e^{x+x^2} &= 1 + x + x^2 + \frac{(x+x^2)^2}{2} + o((x+x^2)^2) = \\ &= 1 + x + x^2 + \frac{x^2 + 2x^3 + x^4}{2} + o(x^2 + 2x^3 + x^4) \\ &= 1 + x + x^2 + \frac{x^2}{2} + o(x^2) \end{aligned}$$

$$\lim_{x \rightarrow -\infty} \sqrt{x^2 + 3x + 2} + x$$

$\swarrow \quad \searrow \quad \swarrow \quad \searrow$
 $+\infty \quad -\infty$

$$\lim_{x \rightarrow -\infty} x^2 + 3x + 2 = \lim_{x \rightarrow -\infty} x^2 \left(1 + \frac{3}{x} + \frac{2}{x^2} \right) = +\infty$$

$\nearrow +\infty$
 $\searrow \quad \swarrow$
 $0 \quad 0$

$$\lim_{x \rightarrow -\infty} \left(\sqrt{x^2 + 3x + 2} + x \right) \cdot \frac{\sqrt{x^2 + 3x + 2} - x}{\sqrt{x^2 + 3x + 2} - x} =$$

$\swarrow \quad \searrow$
 $+\infty \quad +\infty$

$$= \lim_{x \rightarrow -\infty} \frac{x^2 + 3x + 2 - x^2}{\sqrt{x^2 + 3x + 2} - x} = \lim_{x \rightarrow -\infty} \frac{3x + 2}{\sqrt{x^2 \left(1 + \frac{3}{x} + \frac{2}{x^2} \right)} - x} =$$

$$= \lim_{x \rightarrow -\infty} \frac{3x + 2}{|x| \sqrt{1 + \frac{3}{x} + \frac{2}{x^2}} - x} = \lim_{x \rightarrow -\infty} \frac{3x + 2}{-x \sqrt{1 + \frac{3}{x} + \frac{2}{x^2}} - x} =$$

$$= \lim_{x \rightarrow -\infty} \frac{\cancel{x} \left(3 + \frac{2}{\cancel{x}} \right)}{\cancel{x} \left(-\sqrt{1 + \frac{3}{\cancel{x}} + \frac{2}{\cancel{x}^2}} - 1 \right)} = \frac{3}{-1 - 1} = -\frac{3}{2}$$

$\nearrow 0 \quad \searrow 0$

$$|-3| = 3 = -(-3)$$

$$|x| = -x \quad \text{se} \quad x < 0 \quad \nabla \nabla$$

$$|x| = x \quad \text{se} \quad x > 0$$